try indunction principle in Functional_Map_Union_find

MapFind.v
@@ -4,27 +4,84 @@ Require Import Coq.MSets.MSetWeakList.
 Require Import Coq.FSets.FSetFacts.
 Require Import Coq.FSets.FMapAVL.
 Require Import Coq.FSets.FMapFacts.
+Require Import Coq.Program.Equality.
 
 Require Import Top0.Keys.
+Require Import Top0.Definitions.
+Require Import Top0.Nameless.
 
-Inductive type2 :=
-  | Ty2_Natural : type2
-  | Ty2_Boolean : type2.
-
-Definition tau := type2.
-
-Module ST := FMapAVL.Make (RegionVars).
+(*Module ST := FMapAVL.Make (RegionVars).
 Definition Sigma : Type := ST.t tau.
 
 Module STMapP := FMapFacts.Facts ST.
 Module STRaw := ST.Raw.
-Module STProofs := ST.Raw.Proofs.
+Module STProofs := ST.Raw.Proofs.*)
+Module EProofs := ST.Raw.Proofs.
 
-  
 Definition Functional_Map_Union (stty1 stty2 : Sigma) : Sigma :=
   let f := fun (k : nat * nat) (v : tau) (m : Sigma) => ST.add k v m
   in ST.fold f stty1 stty2.
+
+
+(*Lemma StoreTyping_Extended:
+  forall stty sttya sttyb,
+    (forall rho env ctxt, TcEnv (stty, rho, env, ctxt) ) ->
+    (forall (l : ST.key) (t' : tau),
+       ST.find (elt:=tau) l stty = Some t' -> ST.find (elt:=tau) l sttya = Some t' ) ->
+    (forall (l : ST.key) (t' : tau),
+       ST.find (elt:=tau) l stty = Some t' -> ST.find (elt:=tau) l sttyb = Some t' ) ->
+    (forall (l : ST.key) (t' : tau),
+    	ST.find (elt:=tau) l stty = Some t' -> ST.find (elt:=tau) l (Functional_Map_Union sttya sttyb) = Some t' ).
+Proof. 
+  intros stty sttya sttyb Ha Hb.
+  intros l t' H.
+  assert ((forall rho env ctxt, TcEnv (stty, rho, env, ctxt) -> TcEnv (sttya, rho, env, ctxt))) as HA.
+  apply ext_stores__env; auto.
+  assert ((forall rho env ctxt, TcEnv (stty, rho, env, ctxt) -> TcEnv (sttyb, rho, env, ctxt))) as HB.
+  apply ext_stores__env; auto.
+  assert (forall (rho : Rho) (env : Env) (ctxt : Gamma), TcEnv (sttya, rho, env, ctxt)) as HTCEnv_a
+       by (intros; apply HA; auto).
+  assert (forall (rho : Rho) (env : Env) (ctxt : Gamma), TcEnv (sttyb, rho, env, ctxt)) as HTCEnv_b
+       by (intros; apply HB; auto).
+  edestruct HTCEnv_a.
+  unfold ST.find in *.
+  intro.
+  apply EProofs.find_1 with (e:=H) (m:=ST.this (Functional_Map_Union sttya sttyb)) (x:=t').
+  edestruct (Ha l t' H).
+  generalize l. 
+  apply Functional_Map_Union_find.
+Admitted.*)
+
   
-Axiom Functional_Map_Union_find:
+Lemma Functional_Map_Union_find:
   forall sttya sttyb (l : ST.key) (t' : tau),
     ST.find (elt:=tau) l (Functional_Map_Union sttya sttyb) = ST.find (elt:=tau) l sttya.
+Proof.
+  intros.
+  unfold Functional_Map_Union. (*ST.fold.*)
+  destruct sttya. destruct sttyb. simpl. induction this0.
+  - inversion is_bst; subst.
+    + reflexivity. 
+    + unfold ST.find, ST.fold. simpl.
+      destruct ( RegionVars.compare l x); simpl.
+      * admit.
+      * admit.
+      * admit.
+  - inversion is_bst0; subst.
+
+    assert (
+         ST.find (elt:=tau) l
+           (ST.fold (fun (k0 : nat * nat) (v : tau) (m : Sigma) => ST.add k0 v m)
+                    {| ST.this := this; ST.is_bst := is_bst |}
+                    {| ST.this := this0_1; ST.is_bst := H3 |}) =
+           ST.find (elt:=tau) l {| ST.this := this; ST.is_bst := is_bst |}) as HA
+        by (apply IHthis0_1).
+
+   assert (
+         ST.find (elt:=tau) l
+           (ST.fold (fun (k0 : nat * nat) (v : tau) (m : Sigma) => ST.add k0 v m)
+                    {| ST.this := this; ST.is_bst := is_bst |}
+                    {| ST.this := this0_2; ST.is_bst := H5 |}) =
+           ST.find (elt:=tau) l {| ST.this := this; ST.is_bst := is_bst |}) as HB
+       by (apply IHthis0_2).
+Admitted.
